Slight progress on first edges proof.

graph_inst.v
@@ -2,104 +2,149 @@ Set Implicit Arguments.
 Require Import ZArith MSets.
 Require Import mgraphs_ind pair_UOT.
 
-Module mset := MSetAVL.Make PositiveOrderedTypeBits.
-Module NodePair := (PairUsualOrderedType
-                      PositiveOrderedTypeBits PositiveOrderedTypeBits).
-Module msetPair := MSetAVL.Make (NodePair).
-
-Notation node := positive.
-Notation nodePair := NodePair.t.
-Notation node_set := mset.t.
-Notation node_setPair := msetPair.t.
 
 
-Inductive graph : Type :=
-| Empty : graph
-| Node :
-    node -> (** this node's id *)
-    node_set -> (** its neighbors *)
-    graph -> (** the rest of the graph *)
-    graph.
 
-Fixpoint vertices g : node_set :=
-match g with
-| Empty => mset.empty
-| Node x s g' => mset.add x (vertices g')
-end.
 
-Fixpoint edges g : node_setPair :=
-match g with 
-| Empty => msetPair.empty
-| Node x s g' => mset.fold
-                  (fun x' s' => msetPair.add (x,x') s')
-                  s (edges g')
-end.
+
 
 Module Bleh : Graphs PositiveOrderedTypeBits.
-
-Definition t := graph.
-Definition empty := Empty.
-Definition add_vertex : t -> node -> t :=
-  fun t x => Node x mset.empty t.
-Definition add_edge: t -> node * node -> t :=
-  fun g (x : node*node)  =>
-    let (x1, x2) := x in
-      if (mset.mem x1 (vertices g) && mset.mem x2 (vertices g))
-        then Node x1 (mset.add x2 mset.empty) g
-        else g.
   
-Parameter remove_vertex : t -> node -> t.
-Parameter remove_edge : t -> node * node -> t.
+  
+  Module mset := MSetAVL.Make PositiveOrderedTypeBits.
+  Module NodePair := (PairUsualOrderedType
+                        PositiveOrderedTypeBits PositiveOrderedTypeBits).
+  Module msetPair := MSetAVL.Make (NodePair).
 
-Definition vertices : t -> node_set := vertices.
-Definition edges : t -> node_setPair := edges.
-Definition is_vertex : t -> node -> bool :=
-  fun g x => mset.mem x (vertices g).
-Definition is_edge : t -> node * node -> bool :=
-  fun g x => msetPair.mem x (edges g).
-Parameter neighborhood : t -> node -> node_set.
-Lemma empty_vertices : vertices empty = mset.empty.
-Proof. reflexivity. Qed.
-Lemma empty_edges : edges empty = msetPair.empty.
-Proof. reflexivity. Qed.
-Lemma add_vertices :
-  forall (x : node) (g : t), mset.In x (vertices (add_vertex g x)).
-Proof.
-  intros.
-  induction g; simpl; apply mset.add_spec;
-  left; reflexivity.
+
+
+  Definition node := positive.
+  Definition nodePair := NodePair.t.
+  Definition node_set := mset.t.
+  Definition node_setPair := msetPair.t.
+
+  Notation "[ ]" := mset.empty.
+
+  Notation "[ elt0 , .. , eltn ]" := (mset.add elt0 .. (mset.add eltn (mset.empty )) .. ) (at level 60, right associativity).
+
+
+
+  Inductive graph : Type :=
+  | Empty : graph
+  | Node :
+      node -> (** this node's id *)
+      node_set -> (** its neighbors *)
+      graph -> (** the rest of the graph *)
+      graph.
+
+  Fixpoint vertices g : node_set :=
+    match g with
+      | Empty => mset.empty
+      | Node x s g' => mset.add x (vertices g')
+    end.
+
+  Fixpoint edges g : node_setPair :=
+    match g with 
+      | Empty => msetPair.empty
+      | Node x s g' => mset.fold
+                        (fun x' s' => msetPair.add (x,x') s')
+                        s (edges g')
+    end.
+
+
+
+  
+
+  Definition t := graph.
+  Definition empty := Empty.
+  Definition add_vertex : t -> node -> t :=
+    fun t x => Node x mset.empty t.
+  Definition add_edge: t -> node * node -> t :=
+    fun g (x : node*node)  =>
+      let (x1, x2) := x in
+      if (mset.mem x1 (vertices g) && mset.mem x2 (vertices g))
+      then Node x1 ([x2]) g
+      else g.
+  
+  Parameter remove_vertex : t -> node -> t.
+  Parameter remove_edge : t -> node * node -> t.
+
+  
+  
+  Definition is_vertex : t -> node -> bool :=
+    fun g x => mset.mem x (vertices g).
+  Definition is_edge : t -> node * node -> bool :=
+    fun g x => msetPair.mem x (edges g).
+  Parameter neighborhood : t -> node -> node_set.
+  Lemma empty_vertices : vertices empty = mset.empty.
+  Proof. reflexivity. Qed.
+  Lemma empty_edges : edges empty = msetPair.empty.
+  Proof. reflexivity. Qed.
+  Lemma add_vertices :
+    forall (x : node) (g : t), mset.In x (vertices (add_vertex g x)).
+  Proof.
+    intros.
+    induction g; simpl; apply mset.add_spec;
+    left; reflexivity.
+  Qed.
+
+  Lemma add_edges_helper :
+    forall n n0 g,
+       msetPair.In (n, n0) (edges (Node n ([n0]) g)).
+    Proof.
+      intros.
+      induction g.
+      constructor; auto.
+      simpl. rewrite mset.fold_spec.
+      simpl. apply msetPair.add_spec.
+      auto.
 Qed.
-Lemma add_edges :
-  forall (e : node * node) (g : t),
-    mset.In (fst e) (vertices g) ->
-    mset.In (snd e) (vertices g) ->
+  Lemma add_edges :
+    forall (e : node * node) (g : t),
+      mset.In (fst e) (vertices g) ->
+      mset.In (snd e) (vertices g) ->
       msetPair.In e (edges (add_edge g e)).
-Proof.
-  intros. destruct e.
-  induction g; simpl.
-  inversion H.
-  rewrite IHg.
-Admitted.
+  Proof.
+    intros. destruct e.
+    induction g; simpl.
+    inversion H.
+    apply mset.mem_spec in H; apply mset.mem_spec in H0.
+    case_eq (mset.mem n (mset.add n1 (vertices g)));
+    case_eq (mset.mem n0 (mset.add n1 (vertices g))).
+    simpl (_ && _); cbv iota.
+    {
+      intros H1 H2.
+      generalize (Node n1 n2 g).
+      intros. apply msetPair.add_spec.
+      auto.
+    }
+    {
+      intros H1 H2.
+      simpl (_ && _); cbv iota. 
+      
+(* given H and H0 since n and n0 are not in v (g) then they must be equal to n1 and n2 then it should be possible to say that given Node n1 n2 being visible that (n, n0) is in the graph.*)
+      Admitted.
 
-Lemma add_vertices_other :
-  forall (x y : node) (g : t),
-    x <> y -> mset.In y (vertices g) <-> mset.In y (vertices (add_vertex g x)).
-Proof.
-  split; intros; induction g.
-  inversion H0.
-Admitted.
-     Parameter add_edges_other :
-       forall (e1 e2 : node * node) (g : t),
-       e1 <> e2 -> In e2 (edges g) <-> In e2 (edges (add_edge g e1)).
-     Parameter add_vertices_pres_edges :
-       forall (x : node) (g : t), Equal (edges (add_vertex g x)) (edges g).
-     Parameter add_edges_pres_vertices :
-       forall (x : node * node) (g : t),
-       Equal (vertices (add_edge g x)) (vertices g).
-     Parameter remove_vertices :
-       forall (x : node) (g : t), ~ In x (vertices (remove_vertex g x)).
-     Parameter remove_edges :
-       forall (e : node * node) (g : t), ~ In e (edges (remove_edge g e)).
+
+    Lemma add_vertices_other :
+      forall (x y : node) (g : t),
+        x <> y -> mset.In y (vertices g) <-> mset.In y (vertices (add_vertex g x)).
+    Proof.
+      split; intros; induction g.
+      inversion H0.
+    Admitted.
+    Parameter add_edges_other :
+      forall (e1 e2 : node * node) (g : t),
+        e1 <> e2 -> In e2 (edges g) <-> In e2 (edges (add_edge g e1)).
+    Parameter add_vertices_pres_edges :
+      forall (x : node) (g : t), Equal (edges (add_vertex g x)) (edges g).
+    Parameter add_edges_pres_vertices :
+      forall (x : node * node) (g : t),
+        Equal (vertices (add_edge g x)) (vertices g).
+    Parameter remove_vertices :
+      forall (x : node) (g : t), ~ In x (vertices (remove_vertex g x)).
+    Parameter remove_edges :
+      forall (e : node * node) (g : t), ~ In e (edges (remove_edge g e)).
      Parameter remove_vertices_edges_l :
        forall (x1 : node) (g : t) (x2 : node),
        ~ In (x1, x2) (edges (remove_vertex g x1)).
